src/program_proof/tulip/program/gcoord/encode.v
@@ -320,4 +320,29 @@ Section encode.
     by iFrame.
   Qed.
 
+  Theorem wp_EncodeTxnInquireRequest (ts : u64) (rank : u64) :
+    {{{ True }}}
+      EncodeTxnInquireRequest #ts #rank
+    {{{ (dataP : Slice.t) (data : list u8), RET (to_val dataP);
+        own_slice dataP byteT (DfracOwn 1) data ∗
+        ⌜encode_txnreq (InquireReq ts rank) data⌝
+    }}}.
+  Proof.
+    iIntros (Φ) "_ HΦ".
+    wp_rec.
+
+    wp_apply wp_NewSliceWithCap; first word.
+    iIntros (p) "Hbs".
+    wp_apply (wp_WriteInt with "Hbs").
+    iIntros (p1) "Hbs".
+    wp_apply (wp_WriteInt with "Hbs").
+    iIntros (p2) "Hbs".
+    wp_apply (wp_WriteInt with "Hbs").
+    iIntros (p3) "Hbs".
+    wp_pures.
+    rewrite uint_nat_W64_0 replicate_0 app_nil_l -app_assoc.
+    iApply "HΦ".
+    by iFrame.
+  Qed.
+
 End encode.
